@prefix rdf: <http://www.w3.org/1999/02/22-rdf-syntax-ns#> .
@prefix rdfs: <http://www.w3.org/2000/01/rdf-schema#> .
@prefix dcterms: <http://purl.org/dc/terms/> .
@prefix owl: <http://www.w3.org/2002/07/owl#> .
@prefix skos: <http://www.w3.org/2004/02/skos/core#> .
@prefix sssom: <https://w3id.org/sssom/> .
@prefix fair: <https://w3id.org/fair/principles/terms/> .
@prefix dp: <https://data.world/blog/data-product-abcs/#> .

<https://donnywinston.com/fair-vs-data-product-abcde>
    a rdf:Bag ;
    rdfs:subClassOf [
        a owl:Restriction ;
        owl:onProperty rdfs:member ;
        owl:allValuesFrom owl:Axiom ;
    ] ;
    dcterms:title "Mapping FAIR to Data Product ABCs" ;
    skos:note "Thought to make this a https://w3id.org/sssom MappingSet, but that seemed like overkill for now." ;
    skos:relatedMatch <https://w3id.org/sssom/MappingSet> ;
.

<https://www.w3id.org/fair/principles/terms/FAIR-Vocabulary> <http://purl.org/vocab/vann/preferredNamespaceUri> <https://w3id.org/fair/principles/terms/> .

fair:F skos:prefLabel "Findable" .
fair:F1 skos:definition "(meta)data are assigned a globally unique and persistent identifier" .
fair:F2 skos:definition "data are described with rich metadata (defined by R1 below)" .
fair:F3 skos:definition "metadata clearly and explicitly include the identifier of the data it describes" .
fair:F4 skos:definition "(meta)data are registered or indexed in a searchable resource" .

fair:A skos:prefLabel "Accessible" .
fair:A1 skos:definition "(meta)data are retrievable by their identifier using a standardized communications protocol" .
fair:A1.1 skos:definition "the protocol is open, free, and universally implementable" .
fair:A1.2 skos:definition "the protocol allows for an authentication and authorization procedure, where necessary" .
fair:A2 skos:definition "metadata are accessible, even when the data are no longer available" .

fair:I skos:prefLabel "Interoperable" .
fair:I1 skos:definition "(meta)data use a formal, accessible, shared, and broadly applicable language for knowledge representation" .
fair:I2 skos:definition "(meta)data use vocabularies that follow FAIR principles" .
fair:I3 skos:definition "(meta)data include qualified references to other (meta)data" .

fair:R skos:prefLabel "Reusable" .
fair:R1 skos:definition "meta(data) are richly described with a plurality of accurate and relevant attributes" .
fair:R1.1 skos:definition "(meta)data are released with a clear and accessible data usage license" .
fair:R1.2 skos:definition "(meta)data are associated with detailed provenance" .
fair:R1.3 skos:definition "(meta)data meet domain-relevant community standards" .


<https://data.world/blog/data-product-abcs/#> rdfs:isDefinedBy <https://data.world/resources/reports-and-tools/data-mesh-governance-white-paper/> .

dp:aOwns skos:prefLabel "Accountability: Who is the owner that is responsible for the data?" .
dp:aDefines skos:prefLabel "Accountability: Who defines the requirements?" .
dp:aFixes skos:prefLabel "Accountability: Who fixes it when it breaks?" .

dp:aOwns skos:broadMatch fair:R1 .
dp:aDefines skos:broadMatch fair:R1.3 .
dp:aFixes skos:broadMatch fair:R1 .



dp:bWhatIs skos:prefLabel "Boundaries: What is the data?" .
dp:bWhatIsnt skos:prefLabel "Boundaries: What isn't it?" .
dp:bWhere skos:prefLabel "Boundaries: Where will it live?" .
dp:bInsOuts skos:prefLabel "Boundaries: What are the inputs and outputs?" .
dp:bHow skos:prefLabel "Boundaries: How do you balance that roadmap against other organizational priorities and considerations?" .

dp:bWhatIs skos:closeMatch fair:F2, fair:R1 .
dp:bWhatIsnt skos:relatedMatch fair:F2, fair:R1 .
dp:bWhere skos:exactMatch fair:F1 .
dp:bInsOuts skos:closeMatch fair:R1.2 .
dp:bHow skos:relatedMatch fair:I3 .



dp:cData skos:prefLabel "Contracts & Expectations: What are the data constraints, definitions, and tests?" .
dp:cService skos:prefLabel "Contracts & Expectations: What are the SLAs and SLOs?" .
dp:cUse skos:prefLabel "Contracts & Expectations: What are the sharing agreements, consented uses, and policies?" .
dp:cPurpose skos:prefLabel "Contracts & Expectations: What is the purpose?" .
dp:cPerf skos:prefLabel "Contracts & Expectations: What is the performance and scale?" .
dp:cQuality skos:prefLabel "Contracts & Expectations: What are the quality and maintainability details?" .
dp:cSecurity skos:prefLabel "Contracts & Expectations: How is it being kept secure and private? Who can see it? Use it?" .

dp:cData skos:closeMatch fair:I .
dp:cService skos:relatedMatch fair:A, fair:I .
dp:cUse skos:closeMatch fair:R1.1 .
dp:cPurpose skos:relatedMatch fair:F2, fair:R1.3 .
dp:cPerf skos:relatedMatch fair:R .
dp:cQuality skos:relatedMatch fair:R1.2, fair:R1.3 , fair:I3 .
dp:cSecurity skos:narrowMatch fair:A1.2 .



dp:dCurrentConsumers skos:prefLabel "Downstream Consumers: Who are the current consumers?" .
dp:dPotentialConsumers skos:prefLabel "Downstream Consumers: Who are potential consumers?" .
dp:dUseCases skos:prefLabel "Downstream Consumers: What are the use cases that have been considered?" .
dp:dValue skos:prefLabel "Downstream Consumers: What is the value?" .
dp:dRoadmap skos:prefLabel "Downstream Consumers: What is the roadmap of the data product?" .
dp:dEvolvability skos:prefLabel "Downstream Consumers: How will it evolve to provide more value for consumers over time?" .
dp:dUX skos:prefLabel "Downstream Consumers: What is the user experience of the data? APIs, shape, access point?" .

dp:dCurrentConsumers skos:relatedMatch fair:F2, fair:F4, fair:R .
dp:dPotentialConsumers skos:relatedMatch fair:F2, fair:F4, fair:R .
dp:dUseCases skos:relatedMatch fair:R .
dp:dValue skos:relatedMatch fair:R .
dp:dRoadmap skos:relatedMatch fair:I3, fair:R .
dp:dEvolvability skos:relatedMatch fair:I .
dp:dUX skos:relatedMatch fair:A, fair:I .



dp:eMeaning skos:prefLabel "Explicit Knowledge: What is the meaning?" .
dp:eSchema skos:prefLabel "Explicit Knowledge: What is the schema?" .
dp:eRelations skos:prefLabel "Explicit Knowledge: How is it related to other data products?" .
dp:eDocsExamples skos:prefLabel "Explicit Knowledge: Where is the documentation with examples?" .

dp:eMeaning skos:closeMatch fair:I .
dp:eSchema skos:closeMatch fair:I .
dp:eRelations skos:narrowMatch fair:I3 .
dp:eDocsExamples skos:relatedMatch fair:A2, fair:I2, fair:R .